theories/examples.v
@@ -83,30 +83,41 @@ Inductive foo :=
 
 with bar :=
 | Bar1 of foo & foo
-| Bar2 of nat & foo.
+| Bar2 of nat & foo
+
+with baz :=
+| Baz of foo & baz.
 Set Elimination Schemes.
 
 Scheme foo_rect := Induction for foo Sort Type
-with   bar_rect := Induction for bar Sort Type.
+with   bar_rect := Induction for bar Sort Type
+with   baz_rect := Induction for baz Sort Type.
 
-Combined Scheme foo_bar_rect from foo_rect, bar_rect.
+Combined Scheme foo_bar_baz_rect from foo_rect, bar_rect, baz_rect.
 
-Definition foo_bar_mutIndMixin := [mutIndType for foo_bar_rect].
-Canonical foo_indType := IndType _ foo foo_bar_mutIndMixin.
-Canonical bar_indType := IndType _ bar foo_bar_mutIndMixin.
+Definition foo_bar_baz_mutIndMixin := [mutIndType for foo_bar_baz_rect].
+Canonical foo_indType := IndType _ foo foo_bar_baz_mutIndMixin.
+Canonical bar_indType := IndType _ bar foo_bar_baz_mutIndMixin.
+Canonical baz_indType := IndType _ baz foo_bar_baz_mutIndMixin.
 
 Definition foo_eqMixin := [derive lazy eqMixin for foo].
 Canonical foo_eqType := EqType foo foo_eqMixin.
 Definition bar_eqMixin := [derive lazy eqMixin for bar].
 Canonical bar_eqType := EqType bar bar_eqMixin.
+Definition baz_eqMixin := [derive lazy eqMixin for baz].
+Canonical baz_eqType := EqType baz baz_eqMixin.
 Definition foo_choiceMixin := [derive choiceMixin for foo].
 Canonical foo_choiceType := Eval hnf in ChoiceType foo foo_choiceMixin.
 Definition bar_choiceMixin := [derive choiceMixin for bar].
 Canonical bar_choiceType := Eval hnf in ChoiceType bar bar_choiceMixin.
+Definition baz_choiceMixin := [derive choiceMixin for baz].
+Canonical baz_choiceType := Eval hnf in ChoiceType baz baz_choiceMixin.
 Definition foo_countMixin := [derive countMixin for foo].
 Canonical foo_countType := Eval hnf in CountType foo foo_countMixin.
 Definition bar_countMixin := [derive countMixin for bar].
 Canonical bar_countType := Eval hnf in CountType bar bar_countMixin.
+Definition baz_countMixin := [derive countMixin for baz].
+Canonical baz_countType := Eval hnf in CountType baz baz_countMixin.
 Definition foo_orderMixin := [derive lazy orderMixin for foo].
 Canonical foo_porderType := Eval hnf in POrderType tt foo foo_orderMixin.
 Canonical foo_latticeType := Eval hnf in LatticeType foo foo_orderMixin.
@@ -117,6 +128,11 @@ Canonical bar_porderType := Eval hnf in POrderType tt bar bar_orderMixin.
 Canonical bar_latticeType := Eval hnf in LatticeType bar bar_orderMixin.
 Canonical bar_distrLatticeType := Eval hnf in DistrLatticeType bar bar_orderMixin.
 Canonical bar_orderType := Eval hnf in OrderType bar bar_orderMixin.
+Definition baz_orderMixin := [derive lazy orderMixin for baz].
+Canonical baz_porderType := Eval hnf in POrderType tt baz baz_orderMixin.
+Canonical baz_latticeType := Eval hnf in LatticeType baz baz_orderMixin.
+Canonical baz_distrLatticeType := Eval hnf in DistrLatticeType baz baz_orderMixin.
+Canonical baz_orderType := Eval hnf in OrderType baz baz_orderMixin.
 
 End MutualExample.
 
